pass through section 4

soundness.v
@@ -1,10 +1,10 @@
 From WR Require Import syntax join semtyping typing common imports.
 
 (* Semantic substitution well-formedness *)
-Definition γ_ok Γ γ := forall i, i < length Γ -> forall m PA, ⟦ (dep_ith Γ i) [γ] ⟧ m ↘ PA -> PA (γ i).
+Definition ρ_ok Γ ρ := forall i, i < length Γ -> forall m PA, ⟦ (dep_ith Γ i) [ρ] ⟧ m ↘ PA -> PA (ρ i).
 
 (* Semantic typing, written Γ ⊨ a : A in the paper *)
-Definition SemWt Γ a A := forall γ, γ_ok Γ γ -> exists m PA, ( ⟦ A [γ] ⟧ m ↘ PA)  /\ PA (a [γ]).
+Definition SemWt Γ a A := forall ρ, ρ_ok Γ ρ -> exists m PA, ( ⟦ A [ρ] ⟧ m ↘ PA)  /\ PA (a [ρ]).
 Notation "Γ ⊨ a ∈ A" := (SemWt Γ a A) (at level 70).
 
 (* Semantic context wellformedness *)
@@ -13,11 +13,10 @@ Notation "⊨ Γ" := (SemWff Γ) (at level 70).
 
 
 
-Lemma γ_ok_cons {i Γ γ a PA A} :
-  InterpUnivN i (A [γ]) PA ->
-  PA a ->
-  γ_ok Γ γ ->
-  γ_ok (A :: Γ) (a .: γ).
+Lemma ρ_ok_cons {i Γ ρ a PA A} :
+  ⟦ A [ρ] ⟧ i ↘ PA -> PA a ->
+  ρ_ok Γ ρ ->
+  ρ_ok (A :: Γ) (a .: ρ).
 Proof.
   move => h0 h1 h2.
   case => /= [_ | m ? PA0].
@@ -25,45 +24,48 @@ Proof.
     asimpl in hPA0.
     suff : PA = PA0 by congruence.
     hauto l:on use:InterpUnivN_deterministic'.
-  - asimpl. hauto lq:on unfold:γ_ok solve+:lia.
+  - asimpl. hauto lq:on unfold:ρ_ok solve+:lia.
 Qed.
 
-Lemma γ_ok_renaming Γ γ :
+(* Well-formed substitutions are stable under renaming *)
+Lemma ρ_ok_renaming Γ ρ :
   forall Δ ξ,
     good_renaming ξ Γ Δ ->
-    γ_ok Δ γ ->
-    γ_ok Γ (ξ >> γ).
+    ρ_ok Δ ρ ->
+    ρ_ok Γ (ξ >> ρ).
 Proof.
   move => Δ ξ hscope h1.
-  rewrite /γ_ok => i hi j PA.
-  replace (subst_tm (ξ >> γ) (dep_ith Γ i)) with
-    (subst_tm γ (ren_tm ξ (dep_ith Γ i))); last by asimpl.
+  rewrite /ρ_ok => i hi j PA.
+  replace (subst_tm (ξ >> ρ) (dep_ith Γ i)) with
+    (subst_tm ρ (ren_tm ξ (dep_ith Γ i))); last by asimpl.
   rewrite /good_renaming in hscope.
   case /(_ i hi) : hscope => ? h0.
   rewrite -h0 => //.
   by apply h1.
 Qed.
 
+(* Typing is stable under renaming *)
 Lemma renaming_SemWt Γ a A :
-  SemWt Γ a A ->
+  (Γ ⊨ a ∈ A) ->
   forall Δ ξ,
     good_renaming ξ Γ Δ ->
-    SemWt Δ (ren_tm ξ a) (ren_tm ξ A).
+    Δ ⊨ a⟨ξ⟩ ∈ A⟨ξ⟩ .
 Proof.
-  rewrite /SemWt => h Δ ξ hξ γ hγ.
-  have hγ' : (γ_ok Γ (ξ >> γ)) by eauto using γ_ok_renaming.
-  case /(_ _ hγ') : h => PA hPA.
+  rewrite /SemWt => h Δ ξ hξ ρ hρ.
+  have hρ' : (ρ_ok Γ (ξ >> ρ)) by eauto using ρ_ok_renaming.
+  case /(_ _ hρ') : h => PA hPA.
   exists PA. by asimpl.
 Qed.
 
+(* Well-formed types have interpretations *)
 Lemma SemWt_Univ Γ A i :
-  SemWt Γ A (tUniv i) <->
-  forall γ, γ_ok Γ γ -> exists PA , InterpUnivN i (subst_tm γ A) PA.
+  (Γ ⊨ A ∈ tUniv i) <->
+  forall ρ, ρ_ok Γ ρ -> exists S , ⟦ A[ρ] ⟧ i ↘ S.
 Proof.
   rewrite /SemWt.
   split.
   - hauto lq:on rew:off use:InterpUnivN_Univ_inv'.
-  - move => /[swap] γ /[apply].
+  - move => /[swap] ρ /[apply].
     case => PA hPA.
     exists (S i). eexists.
     split.
@@ -71,79 +73,80 @@ Proof.
     + simpl. eauto.
 Qed.
 
+(* Fundamental theorem: Syntactic typing implies semantic typing *)
 Theorem soundness Γ :
-  (forall a A, Wt Γ a A -> SemWt Γ a A) /\
-  (Wff Γ -> SemWff Γ).
+  (forall a A, (Γ ⊢ a ∈ A) -> (Γ ⊨ a ∈ A)) /\
+  ((⊢ Γ) -> (⊨ Γ)).
 Proof.
   move : Γ.
   apply wt_mutual.
-  - move => Γ i h ih ? γ hγ.
+  - move => Γ i h ih ? ρ hρ.
     move /(_ i ltac:(done)) in ih.
     case : ih => F ih.
     suff /SemWt_Univ ih'  : SemWt Γ (dep_ith Γ i) (tUniv (F i)).
-    + move /ih' : (hγ) {ih'} => [PA hPA].
+    + move /ih' : (hρ) {ih'} => [PA hPA].
       exists (F i), PA. sfirstorder.
     + hauto l:on use:dep_ith_shift, good_renaming_truncate, renaming_SemWt.
   - hauto l:on use:SemWt_Univ.
   - move => Γ i A B _ /SemWt_Univ h0 _ /SemWt_Univ h1.
     apply SemWt_Univ.
-    move => γ hγ.
-    move /(_ γ hγ) : h0; intros (PA & hPA).
+    move => ρ hρ.
+    move /(_ ρ hρ) : h0; intros (PA & hPA).
     eexists => /=.
     apply InterpUnivN_Fun_nopf; eauto.
-    move => *; asimpl. eauto using γ_ok_cons.
-  - move => Γ A b B i _ /SemWt_Univ hB _ hb γ hγ.
-    case /(_ γ hγ) : hB => /= PPi hPPi.
+    move => *; asimpl. eauto using ρ_ok_cons.
+  - move => Γ A b B i _ /SemWt_Univ hB _ hb ρ hρ.
+    case /(_ ρ hρ) : hB => /= PPi hPPi.
     exists i, PPi. split => //.
     move /InterpUnivN_Fun_inv_nopf : hPPi.
     intros (PA & hPA & hTot & ?). subst.
     rewrite /ProdSpace.
     move => a PB ha. asimpl => hPB.
-    have : γ_ok (A :: Γ) (a .: γ) by eauto using γ_ok_cons.
+    have : ρ_ok (A :: Γ) (a .: ρ) by eauto using ρ_ok_cons.
     move /hb.
     intros (m & PB0 & hPB0 & hPB0').
     replace PB0 with PB in * by hauto l:on use:InterpUnivN_deterministic'.
     qauto l:on use:P_AppAbs_cbn,InterpUnivN_back_clos  solve+:(by asimpl).
-  - move => Γ f A B b _ ihf _ ihb γ hγ.
+  - move => Γ f A B b _ ihf _ ihb ρ hρ.
     rewrite /SemWt in ihf ihb.
-    move /(_ γ hγ) : ihf; intros (i & PPi & hPi & hf).
-    move /(_ γ hγ) : ihb; intros (j & PA & hPA & hb).
+    move /(_ ρ hρ) : ihf; intros (i & PPi & hPi & hf).
+    move /(_ ρ hρ) : ihb; intros (j & PA & hPA & hb).
     simpl in hPi.
     move /InterpUnivN_Fun_inv_nopf : hPi. intros (PA0 & hPA0 & hTot & ?). subst.
     have ? : PA0 = PA by eauto using InterpUnivN_deterministic'. subst.
     move  : hf (hb). move/[apply].
     move : hTot hb. move/[apply].
     asimpl. hauto lq:on.
-  - move => Γ a A B i _ hA _ /SemWt_Univ hB ? γ hγ.
-    have ? : Coherent (subst_tm γ A) (subst_tm γ B)
+  - move => Γ a A B i _ hA _ /SemWt_Univ hB ? ρ hρ.
+    have ? : Coherent (subst_tm ρ A) (subst_tm ρ B)
       by eauto using Coherent_subst_star.
     qauto l:on use:InterpUnivN_Coherent unfold:SemWt.
   - hauto l:on.
   - hauto l:on.
-  - rewrite /SemWt => Γ a b c A i _ /SemWt_Univ hA _ ha _ hb _ hc γ hγ.
-    case /(_ γ hγ) : ha => ? [PBool [hPBool ha']]; subst.
-    have hγ' : γ_ok (tBool :: Γ) (subst_tm γ a .: γ) by eauto using γ_ok_cons.
+  - rewrite /SemWt => Γ a b c A i _ /SemWt_Univ hA _ ha _ hb _ hc ρ hρ.
+    case /(_ ρ hρ) : ha => ? [PBool [hPBool ha']]; subst.
+    have hρ' : ρ_ok (tBool :: Γ) (subst_tm ρ a .: ρ) by eauto using ρ_ok_cons.
     move /InterpUnivN_Bool_inv : hPBool => ?. subst.
-    case /(_ γ hγ) : hb => ia [PA [hPA hb']].
-    case /(_ γ hγ) : hc => ib [PB [hPB hc']].
-    move : hA hγ'; move/[apply]. move  => [PA0 hPA0].
+    case /(_ ρ hρ) : hb => ia [PA [hPA hb']].
+    case /(_ ρ hρ) : hc => ib [PB [hPB hc']].
+    move : hA hρ'; move/[apply]. move  => [PA0 hPA0].
     exists i, PA0.
     split; first by asimpl.
     case : ha' => v [hred hv].
     asimpl in *.
     case : v hred hv => // ha0 _.
     + move => [:t].
-      apply (InterpUnivN_back_clos_star i) with (A := (subst_tm (tTrue .: γ) A)) (b := (subst_tm γ b)) => //.
+      apply (InterpUnivN_back_clos_star i) with (A := (subst_tm (tTrue .: ρ) A)) (b := (subst_tm ρ b)) => //.
       abstract : t.
-      apply InterpUnivN_preservation_star with (B := subst_tm (tTrue .: γ) A) in hPA0=>//.
+      apply InterpUnivN_preservation_star with (B := subst_tm (tTrue .: ρ) A) in hPA0=>//.
       hauto lq:on ctrs:good_pars_morphing use:pars_morphing_star, good_pars_morphing_ext.
       by apply P_IfTrue_star.
       suff : PA = PA0 by congruence.
       hauto lq:on use:InterpUnivN_deterministic'.
     + move => [:t].
-      apply (InterpUnivN_back_clos_star i) with (A := (subst_tm (tFalse .: γ) A)) (b := (subst_tm γ c)) => //.
+      apply (InterpUnivN_back_clos_star i) with (A := (subst_tm (tFalse .: ρ) A)) (b := (subst_tm ρ c)) => //.
       abstract : t.
-      apply InterpUnivN_preservation_star with (B := subst_tm (tFalse .: γ) A) in hPA0=>//.
+      apply InterpUnivN_preservation_star with (B := subst_tm (tFalse .: ρ) A) in hPA0=>//.
       hauto lq:on ctrs:good_pars_morphing use:pars_morphing_star, good_pars_morphing_ext.
       by apply P_IfFalse_star.
       suff : PB = PA0 by congruence.
@@ -152,31 +155,32 @@ Proof.
   - hauto lq:on use:InterpUnivN_Univ_inv, SemWt_Univ.
   - hauto l:on.
   - hauto l:on use:SemWt_Univ.
-  - move => Γ t a b p A i j C _ _ _ _ _ _ _ hp _ hC _ ht γ hγ.
-    move : hp (hγ); move/[apply] => hp.
-    move : ht (hγ); move/[apply]. intros (m & PA & hPA & ht).
-    have [? [q ?]] : (subst_tm γ p) ⇒* tRefl /\ Coherent (subst_tm γ a) (subst_tm γ b) by
+  - move => Γ t a b p A i j C _ _ _ _ _ _ _ hp _ hC _ ht ρ hρ.
+    move : hp (hρ); move/[apply] => hp.
+    move : ht (hρ); move/[apply]. intros (m & PA & hPA & ht).
+    have [? [q ?]] : (subst_tm ρ p) ⇒* tRefl /\ Coherent (subst_tm ρ a) (subst_tm ρ b) by
       sauto lq:on  rew:db:InterpUniv use:InterpExt_Eq_inv.
     exists m, PA.
     split.
     + asimpl in hPA.
       apply : InterpUnivN_Coherent; eauto.
-      exists (subst_tm (tRefl .: (q .: γ)) C).
+      exists (subst_tm (tRefl .: (q .: ρ)) C).
       hauto lq:on ctrs:good_pars_morphing use:pars_morphing_star, @rtc_refl, good_pars_morphing_ext2.
     + asimpl.
-      eapply InterpUnivN_back_clos_star with (b := subst_tm γ t); eauto.
+      eapply InterpUnivN_back_clos_star with (b := subst_tm ρ t); eauto.
       sfirstorder use: P_JRefl_star.
   - hauto l:on.
 Qed.
 
-Lemma consistency a : ~Wt nil a tVoid.
+(* Void is an empty type *)
+Lemma consistency a : ~ (nil ⊢ a ∈ tVoid).
 Proof.
   move => h.
   apply soundness in h.
   rewrite /SemWt in h.
   move : (h var_tm).
   case.
-  rewrite /γ_ok; sauto lq:on.
+  rewrite /ρ_ok; sauto lq:on.
   asimpl.
   move => i [PA [hPA ha]].
   simp InterpUniv in hPA.
